algunos cambios, pendiente KnapsackVA

src/Especificacion.dfy
@@ -27,29 +27,27 @@ datatype SolutionData = SolutionData(itemsAssign: seq<bool>, k: nat) {
     sum_real(weightsSelected, 0, numSelected)
   }
 
-  ghost function SolutionValue(items: seq<ItemData>): (o: real)
-	requires k <= |items|
-	requires k <= |itemsAssign|
+  ghost function Value(items: seq<ItemData>): (o: real)
+    requires k <= |items|
+    requires k <= |itemsAssign|
   {
-	var objSelected: seq<ItemData> := selectSeq(items, itemsAssign, 0, k);
-	var numSelected: nat := |objSelected|;
-	var valuesSelected: seq<real> := mapSeq(objSelected, (obj: ItemData) => obj.value, 0, numSelected);
-	sum_real(valuesSelected, 0, numSelected)
+    var objSelected: seq<ItemData> := selectSeq(items, itemsAssign, 0, k);
+    var numSelected: nat := |objSelected|;
+    var valuesSelected: seq<real> := mapSeq(objSelected, (obj: ItemData) => obj.value, 0, numSelected);
+    sum_real(valuesSelected, 0, numSelected)
   }
 
-  ghost predicate OptimalSolution(items: seq<ItemData>, itemEndIdx: nat, availableWeight: real, itemsAssign: seq<bool>)
-	requires ValidInstance(items,availableWeight)
-	requires itemEndIdx <= |items|
-	requires itemEndIdx <= |itemsAssign|
-	requires ValidSolution(items, itemEndIdx, availableWeight, itemsAssign)
-{
-	forall otherSolution: seq<bool> | itemEndIdx <= |otherSolution| && ValidSolution(items, itemEndIdx, availableWeight, otherSolution) :: SolutionValue(items, itemEndIdx, otherSolution) <= SolutionValue(items, itemEndIdx, itemsAssign)
-}
+  ghost predicate Optimal(input: InputData)
+    requires this.Valid(input)
+    requires input.Valid()
+  {
+    forall otherSolution: SolutionData | otherSolution.Valid(input) :: otherSolution.Value(input.items) <= Value(input.items)
+  }
 
   ghost predicate Valid(input: InputData){
     0 <= k <= |itemsAssign| &&
     |itemsAssign| == |input.items|
-    && TotalWeight(input.items) <= input.maxWeight    
+    && this.TotalWeight(input.items) <= input.maxWeight
   }
 
 }
