src/Solution.dfy
@@ -1,5 +1,6 @@
 include "Item.dfy"
 include "Especificacion.dfy"
+include "Input.dfy"
 
 class Solution {
   var itemsAssign: array<bool> //objetos seleccionados (si o no)
@@ -14,19 +15,31 @@ class Solution {
     this.k := k';
   }
 
-  ghost predicate Valid (input : InputData)
-    reads this, itemsAssign
+  ghost predicate Valid (input : Input)
+    reads this, itemsAssign, input, input.items
   {
-    && Model().Valid(input) 
-    && Model().TotalWeight(input.items) == totalWeight
-    && Model().SolutionValue(input.items) == totalValue
+    && Model().Valid(input.Model())
+    && Model().TotalWeight(input.Model().items) == totalWeight
+    && Model().Value(input.Model().items) == totalValue
   }
 
-  ghost function Model() : SolutionData 
-  reads this, itemsAssign
+  ghost function Model() : SolutionData
+    reads this, itemsAssign
   {
     SolutionData(itemsAssign[..], k)
   }
+
+  ghost predicate Optimal(input: Input)
+    reads this, itemsAssign, input, input.items
+
+    requires this.Valid(input) // yo como solution debo ser válida
+    requires input.Valid() // la entrada debe ser valida
+  {
+    forall otherSolution: SolutionData | otherSolution.Valid(input.Model()) :: otherSolution.Value(input.Model().items) <= this.Model().Value(input.Model().items)
+  }
+
+  // es correcto lo de arriba? 
+
 
 
 
